bedrock2/src/bedrock2/wsize.v
@@ -1,0 +1,48 @@
+(* Implementation of mulhuu by Andres Erbsen. *)
+
+Require Import bedrock2.NotationsCustomEntry.
+Require Import coqutil.Macros.ident_to_string.
+From bedrock2 Require Import WeakestPrecondition ProgramLogic BasicC64Semantics.
+Require Import bedrock2.ZnWords.
+From Coq Require Import Lia ZArith.
+
+Import bedrock2.Syntax.
+From Coq Require Import BinInt String List Init.Byte. Import ListNotations.
+Import coqutil.Word.Interface coqutil.Word.Properties.
+
+Local Open Scope string_scope.
+Local Open Scope Z_scope.
+Local Open Scope list_scope.
+
+Section WithSemantics.
+Context {width} {BW : Bitwidth.Bitwidth width} {word : word.word width} {word_ok : word.ok word}.
+Context {locals : Interface.map.map string word}.
+Context {mem : Interface.map.map word byte}.
+Context {ext_spec : Semantics.ExtSpec}.
+
+Definition wmask : expr.expr := bedrock_expr:((-$1>>$27)&$63).
+Definition wsize : expr.expr := bedrock_expr:($wmask+$1).
+
+Lemma eval_wmask' : (word.and (word.sru (word.opp (word.of_Z 1)) (word.of_Z 27)) (word.of_Z 63)) = word.of_Z (width-1) :> word.
+Proof.
+  case BW as [ [ -> | -> ] ];
+  apply word.unsigned_inj;
+    rewrite ?word.unsigned_and_nowrap, ?word.unsigned_sru_nowrap, ?word.unsigned_opp;
+    rewrite ?word.unsigned_of_Z; cbv [word.wrap]; cbv; trivial.
+Qed.
+
+Lemma eval_wsize' : word.add (word.and (word.sru (word.opp (word.of_Z 1)) (word.of_Z 27)) (word.of_Z 63)) (word.of_Z 1) = word.of_Z width :> word.
+Proof.
+  case BW as [ [ -> | -> ] ];
+  apply word.unsigned_inj;
+    repeat rewrite ?word.unsigned_and_nowrap, ?word.unsigned_sru_nowrap, ?word.unsigned_opp, ?word.unsigned_add_nowrap;
+    rewrite ?word.unsigned_of_Z; cbv [word.wrap]; cbv; trivial.
+Qed.
+
+Import Map.Interface. (* Coercions *)
+
+Lemma eval_wmask (m : mem) (l : locals) : Semantics.eval_expr m l wmask = Some (word.of_Z (width-1)).
+Proof. cbn. rewrite eval_wmask'; trivial. Qed.
+Lemma eval_wsize (m : mem) (l : locals) : Semantics.eval_expr m l wsize = Some (word.of_Z width).
+Proof. cbn. rewrite eval_wsize'; trivial. Qed.
+End WithSemantics.
